Core/BlockchainProperties.v
@@ -1,0 +1,31 @@
+From mathcomp.ssreflect
+Require Import ssreflect ssrbool ssrnat eqtype ssrfun seq.
+From mathcomp
+Require Import path.
+Require Import Eqdep pred prelude idynamic ordtype pcm finmap unionmap heap coding. 
+Require Import Blockchain.
+Set Implicit Arguments.
+Unset Strict Implicit.
+Unset Printing Implicit Defensive.
+
+Section BlockchainOrder.
+
+Definition is_prefix (bc bc' : Blockchain) :=
+  exists bc1, bc' = bc ++ bc1.
+
+Notation "'[' bc1 '<<=' bc2 ']'" := (is_prefix bc1 bc2).
+
+Lemma bc_pre_refl bc : [bc <<= bc].
+Proof. by exists [::]; rewrite cats0. Qed.
+
+Lemma bc_pre_trans bc1 bc2 bc3 :
+  [bc1 <<= bc2] -> [bc2 <<= bc3] -> [bc1 <<= bc3].
+Proof.
+case=> a1 H1 [a2] H2; subst bc2.
+by rewrite -catA in H2; exists (a1 ++ a2).
+Qed.
+
+End BlockchainOrder.
+
+Notation "'[' bc1 '<<=' bc2 ']'" := (is_prefix bc1 bc2).
+
