PoS/Invariants.v
@@ -2,15 +2,13 @@ From mathcomp.ssreflect
 Require Import ssreflect ssrbool ssrnat eqtype ssrfun seq.
 From mathcomp
 Require Import path.
-Require Import Eqdep pred prelude idynamic ordtype pcm finmap unionmap heap coding. 
-Require Import Blockchain Protocol Semantics States.
+Require Import Eqdep pred prelude idynamic ordtype pcm finmap unionmap heap. 
+Require Import Blockchain Protocol Semantics States BlockchainProperties. 
 Set Implicit Arguments.
 Unset Strict Implicit.
 Unset Printing Implicit Defensive.
 
 (* Invariants of the execution regarding the blockchain *)
-
-
 (* Properties *)
 (*
 Definition holds (n : nid) (w : World) (cond : State -> Prop) :=
@@ -21,19 +19,6 @@ Definition holds (n : nid) (w : World) (cond : State -> Prop) :=
 Definition has_chain (bc : Blockchain) (st : State) : Prop :=
   btChain (blockTree st) == bc.
 
-Lemma has_chain_inj :
-  forall (n : nid) (st: State) (w : World) (bc bc' : Blockchain),
-  find n (localState w) = Some st ->
-  holds n w (has_chain bc) -> holds n w (has_chain bc') -> bc = bc'.
-Proof.
-move=> n st w bc bc' sF nbc nbc'.
-rewrite /holds/has_chain in nbc nbc'.
-specialize (nbc st). specialize (nbc' st). rewrite sF in nbc nbc'.
-assert (Some st = Some st). by [].
-pose proof (nbc H) as nbc. pose proof (nbc' H) as nbc'. clear H.
-move/eqP in nbc. move/eqP in nbc'. rewrite nbc in nbc'. by [].
-Qed.
-
 Definition chain_sync_agreement (w w' : World) :=
   forall (n n' : nid) (bc bc' : Blockchain),
     holds n w (has_chain bc) ->
@@ -42,42 +27,90 @@ Definition chain_sync_agreement (w w' : World) :=
     size bc' == size bc ->
     bc == bc'.
 
+Lemma has_chain_func n w (bc bc' : Blockchain):
+  n \in dom (localState w) ->
+  holds n w (has_chain bc) ->
+  holds n w (has_chain bc') -> bc = bc'.
+Proof.
+case/um_eta=>st[Sf]_ nbc nbc'.
+by move: (nbc st Sf) (nbc' st Sf)=>/eqP<-/eqP->.
+Qed.
+
 (*
 TODO: 
 
 1. Simple property: local BC only grows with stepping;
 2. More complicated: the "rollback" is no more than a contstant;
 
-*)
+ *)
 
-Lemma local_chain_only_grows (w w' : World) :
-  forall (n : nid) (st st' : State) (bc : Blockchain),
-    let: bc' := btChain (blockTree st') in
-    find n (localState w) = Some st ->
-    holds n w (has_chain bc) ->
-    reachable w w' ->
-    find n (localState w') = Some st' ->
-    holds n w' (has_chain bc') ->
-    size bc' <= size bc.
+Lemma local_chain_only_grows_step (w w' : World) n bc bc':
+  n \in dom (localState w) -> 
+  holds n w (has_chain bc) ->
+  system_step w w' ->
+  holds n w' (has_chain bc') ->
+  [bc <<= bc'].
 Proof.
-move=> n st st' bc sF nbc R sF'.
-elim: R st st' bc nbc sF sF' => [|via z S R Hi] st st' bc nbc sF sF' nbc'.
+move=>D H1 S H2; move: (Coh_step S)=>C2.
+case: S=>[[C]Z|
+          p [n' prs bt pool a i] C If F|
+          proc t [n' prs bt pool a i] C F].
 (* 0 steps *)
-- by pose proof (has_chain_inj sF nbc nbc'); rewrite -H; apply leqnn.
-(* Induction over system_steps *)
-- specialize (steps_nodes sF R)=>sFV.
-  specialize (gen_eta sFV). elim. move=> sv. elim. move=> svF _.
-  specialize (Hi st sv bc nbc sF svF). clear st nbc sF sFV.
-  case S. (* Prove for ONE system_step *)
-  + elim. move=> _ vzEq. rewrite vzEq in Hi svF. rewrite svF in sF'.
-    by case: sF'=>eq; rewrite eq in Hi; specialize (Hi nbc').
-  + move=> p ost _ _ _. case (procMsg ost (msg p)).
-    specialize (system_step_local_step S svF sF').
-    (* Prove for induced local transitions *)
-    move=> LS _ _ _. case LS; clear LS ost p.
-    * move=> eq. rewrite eq in svF.
-      specialize (no_change_has_held svF S nbc' sF').
-      move=> h. rewrite -eq in h. specialize (Hi h). rewrite eq in Hi.
-      by apply Hi.
-    (* TODO: Write lemmas for procMsg and procInt *)
-Qed.
+- by subst w'; rewrite (has_chain_func D H1 H2); apply: bc_pre_refl.
+(* Step is procedding a message *)
+
+(* Receiving a message *)
+- have E: (n' = (dst p)) by case:C=>_/(_ (dst p) _ F)/eqP. subst n'.
+
+  (* Two sub-cases: (dst p) =? n *)
+  case N : (n == dst p);[move/eqP:N=>N; subst n|]; last first.
+  (* Message not to us: don't really care about the outcome of procMsg! *)
+  + set pms := (procMsg _ _); case: pms=>st' ms Z; subst w'.
+    rewrite /holds/= findU N/= in H2.
+    by rewrite -(has_chain_func D H1 H2); apply: bc_pre_refl.
+
+    (* Now the interesting case: consider all possible messages, i.e. do
+     case: (msg p). 
+     and prove for each subcase. Perhaps, you might move
+     some parts into lemmas 
+     THIS is the main part of the proof! *)
+  admit.
+
+(* Internal transition *)
+(* Two sub-cases: proc =? n *)
+  case N : (n == proc);[move/eqP:N=>N; subst n|]; last first.
+  set pms := (procInt _ _); case: pms=>st' ms Z; subst w'.
+  rewrite /holds/= findU N/= in H2.
+  by rewrite -(has_chain_func D H1 H2); apply: bc_pre_refl.
+
+(* Another interesting part of the proof:
+   consider all branches in procInt and proof for each one.
+   Don't hesitate to introduce auxiliary lemmas. *)  
+
+Admitted.
+
+(* Big-step case, proven by induction *)
+Lemma local_chain_only_grows (w w' : World) n bc bc':
+  n \in dom (localState w) -> 
+  holds n w (has_chain bc) ->
+  reachable w w' ->
+  holds n w' (has_chain bc') ->
+  [bc <<= bc'].
+Proof.
+move=>D H1 [m]R H2.
+elim: m w' R bc' H2=>/=[w'<-|m Hi w' [via][R S]]bc' H2.
+- by move/(has_chain_func D H1 (bc':=bc')):H2=><-; apply bc_pre_refl.
+have D': n \in dom (localState via).
+- suff R' : reachable w via by rewrite -(steps_nodes R').
+  by exists m. 
+suff X : exists bc1, holds n via (has_chain bc1).
+- case: X=>bc1 H; move: (Hi _ R _ H)=>P.
+  apply: (bc_pre_trans P).
+  apply: (local_chain_only_grows_step D' H S H2).
+rewrite /holds/has_chain.
+move/um_eta: D';case; case=>id ps bt t a i[][->]_.
+by exists (btChain (blockTree {|
+    id := id; peers := ps; blockTree := bt; txPool := t;
+    addr := a; inv := i |}))=>st[]<-. 
+Qed.  
+
